\subsection*{Exercise 13(b)}
We want to find all monic irreducible polynomials of degree $\le 3$ over $\mathbb{Z}_3$. Using this list, we will write the polynomial $f(x) = x^4 + 2x^2 + 2x + 2$ as a product of irreducible polynomials.
\vspace{5mm}

\underline{\textbf{Monic Irreducible Polynomials of Degree $\le 3$ over $\mathbb{Z}_3$}}

\underline{Degree 1} \\
\textit{All polynomials of degree one are irreducible.} \\
$g(x) = x \\
g(x) = x + 1 \\
g(x) = x + 2$

\textit{A polynomial of degree 2 or 3 is irreducible over the field F if and only if it has no roots in F.} \\
\underline{Degree 2} \\
$%g(x) = x^2 \\
g(x) = x^2 + 1 \\
%g(x) = x^2 + 2 \\
%g(x) = x^2 + x \\
%g(x) = x^2 + x + 1 \\
g(x) = x^2 + x + 2 \\
%g(x) = x^2 + 2x \\
%g(x) = x^2 + 2x + 1 \\
g(x) = x^2 + 2x + 2$

\underline{Degree 3} \\
$%g(x) = x^3 \\
%g(x) = x^3 + 1 \\
%g(x) = x^3 + 2 \\
%g(x) = x^3 + x \\
%g(x) = x^3 + x + 1 \\
%g(x) = x^3 + x + 2 \\
%g(x) = x^3 + x^2 \\
%g(x) = x^3 + x^2 + 1 \\
g(x) = x^3 + x^2 + 2 \\
%g(x) = x^3 + x^2 + x \\
%g(x) = x^3 + x^2 + x + 1 \\
g(x) = x^3 + x^2 + x + 2 \\
%g(x) = x^3 + 2x \\
g(x) = x^3 + 2x + 1 \\
g(x) = x^3 + 2x + 2 \\
%g(x) = x^3 + x^2 + 2x \\
g(x) = x^3 + x^2 + 2x + 1 \\
%g(x) = x^3 + x^2 + 2x + 2 \\
%g(x) = x^3 + 2x^2 + 2x \\
%g(x) = x^3 + 2x^2 + 2x + 1 \\
g(x) = x^3 + 2x^2 + 2x + 2 \\
%g(x) = x^3 + 2x^2 \\
g(x) = x^3 + 2x^2 + 1 \\
%g(x) = x^3 + 2x^2 + 2 \\
%g(x) = x^3 + 2x^2 + x \\
g(x) = x^3 + 2x^2 + x + 1 \\
%g(x) = x^3 + 2x^2 + x + 2 
$

Now, we will use the list above to write $f(x)$ as a product of irreducible polynomials. First, notice that $f(2) = 16 + 8 + 4 + 2 = 30 = 0$ over $\mathbb{Z}_3$. Then, by Corollary 4.1.11, $(x - 2)$, or equivalently $(x + 1)$ in $\mathbb{Z}_3[x]$, is a factor of $f(x)$.

\polylongdiv{x^4 + 2x^2 + 2x + 2}{x + 1}

We see that $f(x) = x^4 + 2x^2 + 2x + 2 = (x + 1)(x^3 + 2x^2 + 2)$, which can be reduced further. The quotient $q(x) = x^3 + 2x^2 + 2$ has the root 2, so we proceed similarly:

\polylongdiv{x^3 + 2x^2 + 2}{x + 1}

Now, we have that $f(x) = x^4 + 2x^2 + 2x + 2 = (x + 1)^2(x^2 + x + 2)$.