\subsection*{Exercise 5(b),(d)}
\textbf{(b)}
$f(x) = x^3 - 5x^2 + 6x + 5 \hspace{10mm} c = 2 \hspace{10mm}$ F = $\mathbb{Q} \\
f(2) = (2^3 - 5\cdot2^2 + 6\cdot2 + 5) = (8 - 20 + 12 + 5) = 5$
\begin{align*}
    & f(x) - f(c) = (x^3 - 5x^2 + 6x + 5) - (c^3 - 5c^2 + 6c + 5) \\
    \implies & f(x) - f(2) = (x^3 - 2^3) + (-5x^2 + 5\cdot2^2) + (6x - 6\cdot2) + (5 - 5) \\
    \implies & f(x) - 5 = (x - 2)(x^2 + 2x + 4) - 5(x^2 - 2^2) + 6(x - 2) \\
    \implies & f(x) - 5 = (x - 2)(x^2 + 2x + 4) - 5(x - 2)(x + 2) + 6(x - 2) \\
    \implies & f(x) = (x - 2)[ x^2 + 2x + 4 - 5(x + 2) + 6 ] + 5 \\
    \implies & f(x) = (x - 2)[ x^2 + 2x + 4 - 5x - 10 + 6 ] + 5 \\
    \implies & f(x) = (x - 2)(x^2 - 3x) + 5
\end{align*}
\textbf{(d)}
$f(x) = x^3 + 2x + 3 \hspace{10mm} c = 2 \hspace{10mm}$ F = $\mathbb{Z}_5 \\
f(2) = (2^3 + 2\cdot2 + 3) = (8 + 4 + 3) = 15$
\begin{align*}
    & f(x) - f(c) = (x^3 + 2x + 3) - (c^3 + 2c + 3) \\
    \implies & f(x) - f(2) = (x^3 + 2x + 3) - (2^3 + 2\cdot2 + 3) \\
    \implies & f(x) - 15 = (x^3 - 2^3) + (2x - 2\cdot2) + (3 - 3) \\
    \implies & f(x) - 15 = (x - 2)(x^2 + 2x + 4) + 2(x - 2) \\
    \implies & f(x) = (x - 2)(x^2 + 2x + 4 + 2) + 15 \\
    \implies & f(x) = (x - 2)(x^2 + 2x + 6) + 15 \\
    \implies & f(x) = (x - 2)(x^2 + 2x + 1) \in \mathbb{Z}_5[x]
\end{align*}