\subsection*{Exercise 21(b)}
We want to find the multiplicative inverse of $[a+bx]$ in $\mathbb{Q}[x]/\langle x^2 - 2 \rangle$. The multiplicative inverse of $[a+bx]$ must satisfy the property that $[a+bx][c + dx] = [ac + (ad + bc)x + bdx^2] = [(ac + 2bd) + (ad + bc)x] = [1]$. This implies that $(ac + 2bd) = 1$ and $(ad + bc) = 0$. Then, $(a^2c + 2abd) = a$ and $(abd + b^2c) = 0 \implies c = (\frac{a}{a^2-2b^2})$ and $d = (\frac{-b}{a^2-2b^2})$. Therefore, $[a+bx]^{-1} = [(\frac{a}{a^2-2b^2}) + (\frac{-b}{a^2-2b^2})x] = [\frac{a - bx}{a^2-2b^2}]$.