\subsection*{Exercise 8}
\textit{Let $R$ be a commutative ring such that $a^2 = a$ for all $a \in R$. Show that $a + a = 0$ for all $a \in R$.}

\vspace{5 mm}
For each $a \in R$, we have that $a^2 = a$. Then, $(a + a)^2 = (a + a)(a + a) = a^2 + a^2 + a^2 + a^2$. On the other hand, $(a + a)^2 = (a + a) = (a^2 + a^2)$. But then, this implies that $(a^2 + a^2) = (a^2 + a^2 + a^2 + a^2) \implies 0 = (a^2 + a^2)$ since $R$ is closed under taking additive inverses. But then, we have that $(a + a) = 0$, as desired.