\subsection*{Exercise 1}
Let $p(x,y,z) = 2x^2y - 3xy^3z + 4y^2z^5$ and $q(x,y,z) = 7x^2 + 5x^2y^3z^4 - 3x^2z^3$ be polynomials in $\mathbb{Z}[x,y,z]$.

\vspace{5 mm}
\textbf{[a]}
We write $p$ and $q$ as polynomials in $x$ with coefficients in $\mathbb{Z}[y,z]$. To do this, we treat the indeterminates $y$ and $z$ as coefficients, in addition to treating elements of $\mathbb{Z}$ as coefficients:
\begin{align*}
    p(x) &= (2y)x^2 - (3y^3z)x + (4y^2z^5) \\
    q(x) &= (7 + 5y^3z^4 - 3z^3)x^2
\end{align*}

\vspace{3 mm}
\textbf{[b]} We rewrite the terms of $p(x,y,z)$ and $q(x,y,z)$ in decreasing order with respect to sums of the exponents of the indeterminates $x,y,z$ to determine the degrees of $p$ and $q$:
\begin{align*}
    p(x,y,z) &= 4y^2z^5 - 3xy^3z + 2x^2y \\
    q(x,y,z) &= 5x^2y^3z^4 - 3x^2z^3 + 7x^2
\end{align*}
Notice that the leading term in $p$ is $4y^2z^5 = 4x^0y^2z^5$, which has order $(0 + 2 + 5) = 7$, whereas the remaining terms $(-3xy^3z)$ and $(2x^2y)$ have orders 5 and 3, respectively. On the other hand, the leading term in $q$ is $5x^2y^3z^4$, which has order $(2+3+4)=9$, whereas the remaining terms $(-3x^2z^3)$ and $7x^2$ have orders 5 and 2, respectively. Now, deg($p(x,y,z)) = 7$ and deg($q(x,y,z)) = 9$.

\vspace{5 mm}
\textbf{[c]}
In part (a), we wrote the terms of both $p$ and $q$ in $\mathbb{Z}[y,z]$ in decreasing order with respect to powers of the indeterminate $x$. Therefore, $(2y) \not= 0 \implies$ deg($p(x)) = 2$, and similarly, $(7 + 5y^3z^4 - 3z^3) \not= 0 \implies$ deg($q(x)) = 2$.

Writing $p$ and $q$ as polynomials in $y$ with coefficients in $\mathbb{Z}[x,z]$ in the same manner, we obtain: 
\begin{align*}
    p(y) &= (-3xz)y^3 + (4z^5)y^2 + (2x^2)y \in \mathbb{Z}[x,z] && (-3xz) \not=0 \implies \textnormal{deg}(p(y)) = 3 \\
    q(y) &= (5x^2z^4)y^3 + (-3x^2z^3 + 7x^2) \in \mathbb{Z}[x,z] && (5x^2z^4) \not=0 \implies \textnormal{deg}(q(y)) = 3
\end{align*}
Writing $p$ and $q$ as polynomials in $z$ with coefficients in $\mathbb{Z}[x,y]$ in the same manner, we obtain: 
\begin{align*}
    p(z) &= (4y^2)z^5 - (3xy^3)z + (2x^2y) \in \mathbb{Z}[x,y] && (4y^2) \not=0 \implies \textnormal{deg}(p(z)) = 5 \\
    q(z) &= (5x^2y^3)z^4 - (3x^2)z^3 + (7x^2) \in \mathbb{Z}[x,y] && (5x^2y^3) \not=0 \implies \textnormal{deg}(q(z)) = 4
\end{align*}

\vspace{3 mm}
\textbf{[d]}
Now, we compute $pq \in \mathbb{Z}[x,y,z]$ and find the degrees of the polynomials in each of the three variables $x,y$, and $z$. Ordering terms of $pq$ by decreasing variables' exponential sum, we obtain that deg($pq(x,y,z)) = (2+5+9)=16$.
\begin{align*}
    pq(x,y,z) &= p(x,y,z)\cdot q(x,y,z) \\
    &= (2x^2y - 3xy^3z + 4y^2z^5)\cdot(7x^2 + 5x^2y^3z^4 - 3x^2z^3) \\
    &= (14x^4y + 10x^4y^4z^4 - 6x^4yz^3) - (21x^3y^3z + 15x^3y^6z^5 - 9x^3y^3z^4) + (28x^2y^2z^5 + 20x^2y^5z^9 - 12x^2y^2z^8) \\
    &= 14x^4y + 10x^4y^4z^4 - 6x^4yz^3 - 21x^3y^3z - 15x^3y^6z^5 + 9x^3y^3z^4 + 28x^2y^2z^5 + 20x^2y^5z^9 - 12x^2y^2z^8 \\
    &= 20x^2y^5z^9 - 15x^3y^6z^5 - 12x^2y^2z^8 + 10x^4y^4z^4 + 9x^3y^3z^4 + 28x^2y^2z^5 - 6x^4yz^3 - 21x^3y^3z + 14x^4y
\end{align*}
Writing $pq$ as a polynomial in $x$ with coefficients in $\mathbb{Z}[y,z]$, we obtain that $(14y + 10y^4z^4 - 6yz^3) \not= 0 \implies$ deg($pq(x)) = 4$.

$pq(x) = (14y + 10y^4z^4 - 6yz^3)x^4 - (21y^3z + 15y^6z^5 - 9y^3z^4)x^3 + (28y^2z^5 + 20y^5z^9 - 12y^2z^8)x^2$

\vspace{2 mm}
Writing $pq$ as a polynomial in $y$ with coefficients in $\mathbb{Z}[x,z]$, we have $(15x^3z^5) \not= 0 \implies$ deg($pq(y)) = 6$.
$$pq(y) = (-15x^3z^5)y^6 + (20x^2z^9)y^5 + (10x^4z^4)y^4 - (21x^3z + 9x^3z^4)y^3 + (28x^2z^5 - 12x^2z^8)y^2 + (14x^4 - 6x^4z^3)y$$

Writing $pq$ as a polynomial in $z$ with coefficients in $\mathbb{Z}[x,y]$, we have $(20x^2y^5) \not= 0 \implies$ deg($pq(z)) = 9$.
$$pq(z) = (20x^2y^5)z^9 - (12x^2y^2)z^8 + (28x^2y^2 - 15x^3y^6)z^5 + (10x^4y^4 + 9x^3y^3)z^4 - (6x^4y)z^3 -  (21x^3y^3)z + (14x^4y)$$

\vspace{5 mm}
\textbf{[e]}
Writing $pq$ as a polynomial in $z$ with coefficients in $\mathbb{Z}[x,y]$, we obtain, as in part (d), that $pq(z) = (20x^2y^5)z^9 - (12x^2y^2)z^8 + (28x^2y^2 - 15x^3y^6)z^5 + (10x^4y^4 + 9x^3y^3)z^4 - (6x^4y)z^3 -  (21x^3y^3)z + (14x^4y)$.